Simplify/remove assumptions on clos_callProof

compiler/backend/proofs/clos_callProofScript.sml
@@ -1873,6 +1873,12 @@ val code_inv_def = Define `
              every_Fn_vs_NONE exp /\
              ALL_DISTINCT (code_locs exp))`
 
+val dummy_code_inv = mk_var("code_inv",
+  type_of(#1(strip_comb(lhs(concl(SPEC_ALL code_inv_def))))))
+val code_inv_def = Define`
+  ^dummy_code_inv g1_opt s_code
+     s_cc s_co t_code t_cc t_co ⇔ (s_code = FEMPTY)`;
+
 val SUBMAP_FUPDATE_LIST = Q.store_thm("SUBMAP_FUPDATE_LIST",
   `!f xs. ALL_DISTINCT (MAP FST xs) ∧ DISJOINT (FDOM f) (set (MAP FST xs)) ⇒ f SUBMAP (f |++ xs)`,
   Induct_on`xs` \\ simp[FORALL_PROD] \\ rw[FUPDATE_LIST_THM]
@@ -1886,6 +1892,12 @@ val includes_state_def = Define `
   includes_state g1 s_compile_oracle <=>
     ?k:num. FST (FST (s_compile_oracle k)) = FST g1`;
 
+val dummy_includes_state = mk_var("includes_state",
+  type_of(#1(strip_comb(lhs(concl(SPEC_ALL includes_state_def))))))
+val includes_state_def = Define`
+  ^dummy_includes_state g1_s compile_oracle ⇔ T`;
+
+(*
 val code_rel_state_rel_install = store_thm("code_rel_state_rel_install",
   ``code_inv (SOME g1)
       r.code r.compile r.compile_oracle t.code t.compile t.compile_oracle /\
@@ -2013,6 +2025,7 @@ val code_rel_state_rel_install = store_thm("code_rel_state_rel_install",
   \\ fs [MEM_MAP] \\ rename [`MEM kk _`]
   \\ PairCases_on `kk` \\ rveq \\ fs []
   \\ fs [MEM_toAList,SUBSET_DEF,PULL_EXISTS,ADD1,FLOOKUP_DEF,domain_lookup]) |> GEN_ALL;
+*)
 
 val fv_GENLIST_Var_alt = store_thm("fv_GENLIST_Var_alt",
   ``∀n i tra. fv v (GENLIST_Var tra i n) ⇔ v < n``,
@@ -4108,13 +4121,19 @@ val semantics_calls = Q.store_thm("semantics_calls",
   \\ rpt (disch_then drule) \\ fs [EVAL ``wfg (LN,[])``]
   \\ ntac 2 (pop_assum mp_tac)
   \\ simp [Once code_inv_def]
-  \\ ntac 2 strip_tac
+  \\ (*ntac 2*) strip_tac
   \\ drule evaluate_code
   \\ strip_tac \\ fs [initial_state_def]
+  (*
   \\ disch_then (qspecl_then [`[]`,
       `initial_state ffi max_app (FOLDL $|+ FEMPTY aux) co1 cc1 k`,
       `UNIV DIFF domain (FST (FST (s2.compile_oracle 0)))`,
       `full_gs n`] mp_tac)
+  *)
+  \\ disch_then (qspecl_then [`[]`,
+      `initial_state ffi max_app (FOLDL $|+ FEMPTY aux) co1 cc1 k`,
+      `UNIV DIFF domain (FST (FST (co 0)))`,
+      `FST (FST (co 0)),aux`] mp_tac)
   \\ simp []
   \\ `wfg (FST (FST (co 0)),aux)` by
    (match_mp_tac calls_wfg
@@ -4131,12 +4150,14 @@ val semantics_calls = Q.store_thm("semantics_calls",
     \\ fs [state_rel_def]
     \\ Cases_on `res1` \\ fs []
     \\ Cases_on `e` \\ fs [])
-  \\ rpt conj_tac
   \\ fs [env_rel_def,state_rel_def,initial_state_def,code_includes_def]
+  (*
   \\ `FST (FST (shift_seq n co 0)) = FST (full_gs n)` by
        metis_tac [co_ok_IMP_full_gs_eq_shift_seq]
+  *)
   \\ fs [correct_l_def]
-  THEN1 (fs [wfv_state_def,initial_state_def,FEVERY_DEF,code_inv_def])
+  \\ conj_tac THEN1 (fs [wfv_state_def,initial_state_def,FEVERY_DEF,code_inv_def])
+  (*
   THEN1
    (match_mp_tac subg_trans
     \\ qexists_tac `full_gs 0`
@@ -4147,14 +4168,20 @@ val semantics_calls = Q.store_thm("semantics_calls",
     \\ strip_tac \\ imp_res_tac make_g_wfg
     \\ imp_res_tac make_g_subg
     \\ fs [FUPDATE_LIST])
-  THEN1
+  *)
+  \\ conj_tac THEN1 (
+    match_mp_tac subg_refl
+    \\ fs[] \\ fs[wfg_def] )
+  \\ conj_tac THEN1
    (fs [SUBSET_DEF]
     \\ drule evaluate_code \\ strip_tac
     \\ fs [shift_seq_def,extra_code_assum_def]
     \\ metis_tac [])
-  THEN1 (fs [IN_DISJOINT,IN_DIFF,shift_seq_def])
-  THEN1 (metis_tac [co_ok_IMP_wfg_full_gs])
-  THEN1
+  \\ conj_tac THEN1 (fs [IN_DISJOINT,IN_DIFF,shift_seq_def])
+  (*
+  \\ conj_tac THEN1 (metis_tac [co_ok_IMP_wfg_full_gs])
+  *)
+  \\ conj_tac THEN1
    (full_simp_tac std_ss [GSYM FUPDATE_LIST]
     \\ rpt strip_tac
     \\ match_mp_tac mem_to_flookup
@@ -4163,7 +4190,7 @@ val semantics_calls = Q.store_thm("semantics_calls",
     \\ pop_assum (fn th => once_rewrite_tac [th])
     \\ match_mp_tac calls_ALL_DISTINCT
     \\ asm_exists_tac \\ fs [])
-  THEN1 (fs [code_inv_def] \\ metis_tac [])
+  \\ conj_tac THEN1 (fs [code_inv_def] \\ metis_tac [])
   \\ fs [includes_state_def] \\ qexists_tac `0` \\ fs []);
 
 val semantics_compile = Q.store_thm("semantics_compile",
@@ -4225,6 +4252,7 @@ val ALL_DISTINCT_make_gs = store_thm("ALL_DISTINCT_make_gs",
     \\ imp_res_tac make_g_wfg \\ fs [wfg_def])
   \\ rpt (pairarg_tac \\ fs []));
 
+(*
 val ALOOKUP_make_gs = store_thm("ALOOKUP_make_gs",
   ``!i v code co2.
        (∀k. IS_SOME (make_gs code co2 k)) /\
@@ -4250,6 +4278,7 @@ val ALOOKUP_make_gs = store_thm("ALOOKUP_make_gs",
   \\ qexists_tac `k'` \\ fs []
   \\ rveq \\ fs []
   \\ cheat (* this proof needs a slightly different approach *));
+*)
 
 val FST_THE_make_gs = store_thm("FST_THE_make_gs",
   ``!k code co2.
@@ -4258,6 +4287,7 @@ val FST_THE_make_gs = store_thm("FST_THE_make_gs",
   Induct \\ fs [make_gs_def,make_g_def] \\ rw []
   \\ rpt (pairarg_tac \\ fs []) \\ fs [shift_seq_def,ADD1]);
 
+(*
 val IMP_co_ok = store_thm("IMP_co_ok",
   ``!code co2 k.
       (!i. let (cfg,exp,aux) = co2 i in
@@ -4338,6 +4368,7 @@ val IMP_co_ok = store_thm("IMP_co_ok",
   \\ fs [compile_inc_def]
   \\ rpt (pairarg_tac \\ fs []) \\ rveq \\ fs []
   \\ imp_res_tac calls_subspt \\ fs []);
+*)
 
 (* Preservation of some label properties
   every_Fn_SOME xs ∧ every_Fn_vs_NONE xs
